CC/Subtype/TypeSubst.lean
@@ -43,6 +43,8 @@ def SubtypeP.tsubst'
     apply Subcapt.tsubst <;> trivial
     rename_i ih _ _ _ _ _
     apply ih <;> trivial
+  case cap =>
+    unfold tsubst_motive_ctype at *; intros; simp [CType.tsubst]; constructor
   case refl =>
     unfold tsubst_motive; intros
     apply SubtypeP.refl
@@ -95,7 +97,7 @@ def Subtype.tsubst
   (σ : VarTypeMap Γ Δ g)
   (δ : TVarSubst Γ Δ g) :
   Subtype Δ (T1.tsubst g) (T2.tsubst g) := by
-  cases h
+  cases h <;> try (solve | simp [CType.tsubst]; constructor)
   constructor
   apply Subcapt.tsubst <;> trivial
   apply SubtypeP.tsubst <;> trivial
